extraction/theories/UnivSubst.v
@@ -21,19 +21,19 @@ Fixpoint subst_instance_constr (u : universe_instance) (c : term) :=
   | tConst c u' => tConst c (UnivSubst.subst_instance_instance u u')
   | tConstruct ind k u' => tConstruct ind k (UnivSubst.subst_instance_instance u u')
   | tEvar ev args => tEvar ev (List.map (subst_instance_constr u) args)
-  | tLambda na T M => tLambda na (subst_instance_constr u T) (subst_instance_constr u M)
+  | tLambda na M => tLambda na (subst_instance_constr u M)
   | tApp f v => tApp (subst_instance_constr u f) (subst_instance_constr u v)
-  | tLetIn na b ty b' => tLetIn na (subst_instance_constr u b) (subst_instance_constr u ty)
+  | tLetIn na b b' => tLetIn na (subst_instance_constr u b)
                                 (subst_instance_constr u b')
-  | tCase ind p c brs =>
+  | tCase ind c brs =>
     let brs' := List.map (on_snd (subst_instance_constr u)) brs in
-    tCase ind (subst_instance_constr u p) (subst_instance_constr u c) brs'
+    tCase ind (subst_instance_constr u c) brs'
   | tProj p c => tProj p (subst_instance_constr u c)
   | tFix mfix idx =>
-    let mfix' := List.map (map_def (subst_instance_constr u) (subst_instance_constr u)) mfix in
+    let mfix' := List.map (map_def (subst_instance_constr u)) mfix in
     tFix mfix' idx
   | tCoFix mfix idx =>
-    let mfix' := List.map (map_def (subst_instance_constr u) (subst_instance_constr u)) mfix in
+    let mfix' := List.map (map_def (subst_instance_constr u)) mfix in
     tCoFix mfix' idx
   end.
 
